{
 "cells": [
  {
   "cell_type": "markdown",
   "id": "ec9b1952",
   "metadata": {},
   "source": [
    "# 1D Heat Equation in an Infinite Solid\n",
    "Consider the energy equation,\n",
    "\n",
    "$$\\ \\rho C_p\\displaystyle \\frac{\\partial^{}T}{\\partial t ^{}}+\\rho C_p\\mathbf{v}\\cdot\\nabla T =k\\nabla^2T + q +\\Phi,$$\n",
    "\n",
    "there is no convection in a solid, thus $\\mathbf{v}=\\mathbf{0}$, there\n",
    "is also no viscous dissipation, thus, $\\Phi=0$. Dividing the resulting\n",
    "equation by $\\rho C_p$, we arrive at the famous Fourier heat equation,\n",
    "\n",
    "$$\\ \\displaystyle \\frac{\\partial^{}T}{\\partial t ^{}} = \\alpha\\nabla^2T + Q,$$\n",
    "\n",
    "where $\\alpha=\\rho C_p/k$ is the thermal diffusivity and\n",
    "$Q = q/\\rho C_p$ is the modified heat source.\n",
    "\n",
    "The problem we wish to consider is heat conduction in an infinite solid\n",
    "where energy can enter the system through the heat source, $Q$.\n",
    "Physically, this problem would arise in a long metal rod that can be\n",
    "approximated as infinitely long. The rod must also have a high thermal\n",
    "conductivity or a be very thin in order to approximate that the heat\n",
    "conduction is only occurring in the lateral direction.\n",
    "\n",
    "## 1D Heat Equation Over the Real Line\n",
    "\n",
    "Mathematically, we have the problem, \n",
    "$$\\ T_t-\\alpha T_{xx}=Q(x,t),$$\n",
    "\n",
    "$$\\ T \\to T_{\\infty} \\ \\text{as}\\ x\\to\\infty,$$\n",
    "\n",
    "$$\\ T(x,0)=T_0(x),$$\n",
    "\n",
    "where subscript denotes partial differentiation, $T_{\\infty}$ is the\n",
    "temperature of the rod at an infinite distance from the center, and\n",
    "$T_0(x)$ is the initial temperature distribution. The boundary condition\n",
    "arises because we cannot have a non-zero flux at an infinite distance,\n",
    "otherwise, the rod would have an infinite energy. To normalize the\n",
    "problem, we introduce new variables, $u$ and $f$, defined by,\n",
    "\n",
    "$$\\ u(x,t) = T - T_{\\infty},$$\n",
    "\n",
    "$$\\ f(x) = T_0(x) - T_{\\infty}.$$\n",
    "\n",
    "Plugging this back into the PDE and conditions results in,\n",
    "\n",
    "$$\\ u_t-\\alpha u_{xx}=Q(x,t),$$\n",
    "\n",
    "$$\\ u \\to 0 \\ \\text{as}\\ x\\to\\infty,$$\n",
    "\n",
    "$$\\ u(x,0)=f(x),$$ \n",
    "\n",
    "Owing to the infinite spacial domain, we may wish to\n",
    "consider taking the Fourier Transform of the PDE. If we take the Fourier\n",
    "Transform in $x$, we have,\n",
    "\n",
    "$$\\ \\hat{u}_t+\\alpha\\omega^2\\hat{u}=\\hat{Q},$$ \n",
    "\n",
    "where,\n",
    "\n",
    "$$\\ \\hat{u}(\\omega, t)=\\mathcal{F}\\left\\{ u \\right\\}=\\frac{1}{\\sqrt{2\\pi}}\\int_{\\mathbb{R}^{}} u(x,t) e^{-i\\omega x}dx,$$\n",
    "\n",
    "$$\\ \\hat{Q}(\\omega, t)=\\mathcal{F}\\left\\{ Q \\right\\}=\\frac{1}{\\sqrt{2\\pi}}\\int_{\\mathbb{R}^{}} Q(x,t) e^{-i\\omega x}dx,$$\n",
    "\n",
    "$$\\ \\hat{f}(\\omega)=\\mathcal{F}\\left\\{ f \\right\\}=\\frac{1}{\\sqrt{2\\pi}}\\int_{\\mathbb{R}^{}} f(x) e^{-i\\omega x}dx,$$\n",
    "\n",
    "and we have used the property (integration by parts),\n",
    "\n",
    "$$\\ \\mathcal{F}\\left\\{ u_{xx} \\right\\}=(i\\omega)^2\\mathcal{F}\\left\\{ u \\right\\}.$$\n",
    "\n",
    "This transformation has reduced the PDE into a simple ODE in $t$. By\n",
    "multiplying by an integrating factor, $\\mu$,\n",
    "\n",
    "$$\\ \\mu=e^{\\alpha\\omega^2t},$$ we can rewrite the transformed PDE as,\n",
    "\n",
    "$$\\ \\displaystyle \\frac{d^{}}{dt^{}}\\left(\\hat{u}e^{\\alpha\\omega^2 t}\\right)=\\hat{Q}e^{\\alpha\\omega^2 t}$$\n",
    "\n",
    "$$\\ \\implies \\hat{u}=\\hat{f}e^{-\\alpha\\omega^2t} + \\int_0^t\\hat{Q}(\\omega,\\tau)e^{-\\alpha\\omega^2(t-\\tau)}d\\tau.$$\n",
    "\n",
    "The inverse transform can be symbolically solved using the convolution\n",
    "property and the inverse transform of a Gaussian (shown proceeding this\n",
    "section),\n",
    "\n",
    "$$\\ \\mathcal{F}^{-1}\\left\\{ \\hat{p}\\hat{q} \\right\\}=\\frac{1}{\\sqrt{2\\pi}}\\,p\\ast q.$$\n",
    "\n",
    "Thus we have a symbolic solution,\n",
    "\n",
    "$$\\ u(x,t)=\\frac{f(x)}{\\sqrt{2\\pi}}\\ast\\mathcal{F}^{-1}\\left\\{ e^{-\\alpha\\omega^2t} \\right\\}+\\frac{1}{\\sqrt{2\\pi}}\\int_0^t \n",
    "Q(x,\\tau)\\ast\\mathcal{F}^{-1}\\left\\{ e^{-\\alpha\\omega^2(t-\\tau)} \\right\\} d\\tau\\,$$\n",
    "\n",
    "or more explicitly,\n",
    "\n",
    "$$\\ u(x,t)=\\frac{1}{\\sqrt{4\\pi \\alpha t}}\\int_{\\mathbb{R}^{}}f(y)\\exp{\\left(-\\frac{(x-y)^2}{4\\alpha t}\\right)}dy$$\n",
    "\n",
    "$$\\ +\\int_0^t\\frac{1}{\\sqrt{4\\pi \\alpha(t-\\tau)}}\\int_{\\mathbb{R}^{}}Q(y,\\tau)\\exp{\\left(-\\frac{(x-y)^2}{4\\alpha(t-\\tau)}\\right)}dyd\\tau.$$\n",
    "\n",
    "The first term accounts for propagation of the initial condition through\n",
    "the solution while the second term accounts for the contribution of the\n",
    "heat source to the solution. As $t\\to 0$ the Gaussian 'kernel' converges\n",
    "to $\\delta(x-y)$ as the standard deviation of the Gaussian approaches 0.\n",
    "In PDE theory, it is useful to define the fundamental solution, $\\Phi$,\n",
    "also called a Green's function, $G$,\n",
    "\n",
    "$$\\ \\Phi(x,t,y,\\tau)=G(x,t,y,\\tau)=\\frac{1}{\\sqrt{4\\pi \\alpha(t-\\tau)}}\\exp{\\left(-\\frac{(x-y)^2}{4\\alpha(t-\\tau)}\\right)}.$$\n",
    "\n",
    "Thus, the solution can be written as,\n",
    "\n",
    "$$\\ u(x,t) = \\int_{\\mathbb{R}^{}}f(y)\\Phi(x,t,y,0)\\,dy + \\int_0^t\\int_{\\mathbb{R}^{}}Q(y,\\tau)\\Phi(x,t,y,\\tau)\\,dyd\\tau.$$\n",
    "\n",
    "Essentially, $\\Phi$ captures the evolution of the PDE which is summed\n",
    "(integrated) against the heat source to propagate its effect through the\n",
    "PDE. Fundamental solutions are a rich topic in modern PDE theory, but\n",
    "are rarely used in practical solutions to PDE's as finding fundamental\n",
    "solutions becomes much harder for more complex PDE's. In the rare case\n",
    "that $\\Phi$ can be calculated, the Boundary Element Method offers a\n",
    "powerful numerical solution technique to solve a PDE based solely on the\n",
    "boundary information.\n",
    "\n",
    "## Inverse Fourier Transform of a Gaussian \n",
    "We wish to calculate,\n",
    "\n",
    "$$\\ \\mathcal{F}^{-1}\\left\\{ e^{-\\alpha\\omega^2t} \\right\\}=\\frac{1}{\\sqrt{2\\pi}}\\int_{\\mathbb{R}^{}}{e^{-\\alpha \\omega^2t+i\\omega x}}d\\omega,$$\n",
    "\n",
    "which can be done by completing the square on,\n",
    "\n",
    "$$\\ -k\\omega^2t+i\\omega x$$\n",
    "\n",
    "$$\\ =\\left(\\sqrt{kt}i\\omega+\\frac{1}{2\\sqrt{kt}}x\\right)^2-\\frac{x^2}{4kt}.$$\n",
    "\n",
    "Thus, plugging in this manipulation,\n",
    "\n",
    "$$\\ \\mathcal{F}^{-1}\\left\\{ e^{-k\\omega^2t} \\right\\}=\\frac{e^{-\\frac{x^2}{4\\alpha t}}}{\\sqrt{2\\pi}}\\int_{\\mathbb{R}^{}} e^{\\left(\\sqrt{kt}i\\omega+\\frac{1}{2\\sqrt{\\alpha t}}x\\right)^2} d\\omega.$$\n",
    "\n",
    "Letting, \n",
    "\n",
    "$$\\ iz=\\sqrt{\\alpha t}i\\omega+\\frac{1}{2\\sqrt{\\alpha t}}x,$$\n",
    "and, \n",
    "\n",
    "$$\\ \\frac{dz}{\\sqrt{kt}}=d\\omega,$$ \n",
    "\n",
    "we have,\n",
    "\n",
    "$$\\ \\mathcal{F}^{-1}\\left\\{ e^{-\\alpha\\omega^2t} \\right\\}=\\frac{e^{-\\frac{x^2}{4\\alpha t}}}{\\sqrt{2\\pi kt}}\\int_{-\\infty-\\frac{ix}{2\\sqrt{\\alpha t}}}^{\\infty-\\frac{ix}{2\\sqrt{\\alpha t}}}e^{-z^2}dz.$$\n",
    "\n",
    "The remaining integral requires calculus in the complex plane (complex\n",
    "analysis), but in short, it evaluates to the Gaussian integral,\n",
    "$\\sqrt{\\pi}$, giving,\n",
    "\n",
    "$$\\ \\mathcal{F}^{-1}\\left\\{ e^{-\\alpha\\omega^2t} \\right\\}=\\frac{e^{-\\frac{x^2}{4\\alpha t}}}{\\sqrt{2\\alpha t}}.$$\n",
    "\n",
    "In more detail, the integral is taken over a contour, $\\Gamma$, which\n",
    "further decompose into 4 curves, \n",
    "\n",
    "$$\\ \\Gamma = c_1 + c_2 + c_3 + c_4,$$\n",
    "\n",
    "Since $\\exp{\\left(-z^2\\right)}$ is an 'analytic' function (has a\n",
    "convergent Taylor Series), a theorem called the Cauchy-Goursat Theorem\n",
    "implies that any closed path integral in the complex plane evaluates to\n",
    "0. This theorem is essentially a complex version of the Gradient Theorem\n",
    "from multivariable calculus and the Fundamental Theorem of Calculus from\n",
    "single variable calculus. We thus now have,\n",
    "\n",
    "$$\\ \\int_{c_1}e^{-z^2}\\, dz + \\int_{c_2}e^{-z^2}\\, dz + \\int_{c_3}e^{-z^2}\\, dz + \\int_{c_4}e^{-z^2}\\, dz = 0.$$\n",
    "\n",
    "Let's first consider the integral over $c_2$ and $c_4$. We let,\n",
    "\n",
    "$$\\ a = \\frac{x}{2\\sqrt{\\alpha t}},$$ \n",
    "\n",
    "giving,\n",
    "\n",
    "$$\\ \\int_{c_2}e^{-z^2}\\, dz =I_2= \\lim_{R\\to\\infty}\\int_{R-ia}^{R}e^{-z^2}\\, dz,$$\n",
    "\n",
    "$$\\ \\int_{c_4}e^{-z^2}\\, dz =I_4= \\lim_{L\\to\\infty}\\int^{L-ia}_{L}e^{-z^2}\\, dz.$$\n",
    "\n",
    "We will only consider the integral over $I_2$ since $I_2$ and $I_4$\n",
    "nearly identical. Notice the along $c_2$, \n",
    "\n",
    "$$\\ z = R + iy,$$ \n",
    "\n",
    "and,\n",
    "\n",
    "$$\\ dz = idy,$$ \n",
    "\n",
    "for $-a \\le y\\le 0$. Thus, \n",
    "\n",
    "$$\\begin{aligned}\n",
    "    I_2 &= \\lim_{R\\to\\infty}i\\int_{R-ia}^{R}e^{-(R+iy)^2}\\, dy\\\\\n",
    "    &= \\lim_{R\\to\\infty}i\\int_{R-ia}^{R}e^{-R^2-2Ryi+y^2}\\, dy\\\\\n",
    "\\end{aligned}$$ \n",
    "\n",
    "taking the magnitude of both sides,\n",
    "\n",
    "$$\\ \\left|I_2\\right| = \\lim_{R\\to\\infty} \\left|\\int_{R-ia}^{R}e^{-R^2-2Ryi+y^2}\\, dy\\right|.$$\n",
    "\n",
    "We wish to get an estimate of $\\left|I_2\\right|$, we may use the the\n",
    "Cauchy-Schwartz inequality for this,\n",
    "\n",
    "$$\\ \\left|\\int_{R-ia}^{R}e^{-R^2-2Ryi+y^2}\\, dy\\right| \\le \\left|\\int_{R-ia}^{R}e^{-R^2}\\, dy\\right|\\left|\\int_{R-\n",
    "ia}^{R}e^{-2Ryi}\\, dy\\right|\\left|\\int_{R-ia}^{R}e^{y^2}\\, dy\\right|.$$\n",
    "\n",
    "The first term is, \n",
    "\n",
    "$$\\begin{aligned}\n",
    "    \\left|\\int_{R-ia}^{R}e^{-R^2}\\, dy\\right| &= \\left|e^{-R^2}\\left(R-R+ia\\right)\\right|\\\\\n",
    "    & = a e^{-R^2}.\n",
    "\\end{aligned}$$ \n",
    "\n",
    "The second term is (by the triangle inequality),\n",
    "\n",
    "$$\\begin{aligned}\n",
    "    \\left|\\int_{R-ia}^{R}e^{-2Ryi}\\, dy\\right| &\\le \\left|\\int_{R-ia}^{R}\\left|e^{-2Ryi}\\right|\\, dy\\right|\\\\\n",
    "    & = \\left|\\left(R-R+ia\\right)\\right|\\\\\n",
    "    & = a,\n",
    "\\end{aligned}$$ \n",
    "\n",
    "where $\\left|e^{-2Ryi}\\right|=1$ since $-2Ryi$ is a pure\n",
    "phase with no real part. Finally, the third integral is,\n",
    "\n",
    "$$\\begin{aligned}\n",
    "    \\left|\\int_{R-ia}^{R}e^{y^2}\\, dy\\right| &\\le \\left|\\int_{R-ia}^{R}e^{a^2}\\, dy\\right|\\\\\n",
    "    & = \\left|e^{a^2}\\left(R-R+ia\\right)\\right|\\\\\n",
    "    & = a e^{a^2},\n",
    "\\end{aligned}$$ \n",
    "\n",
    "where we have used the fact that\n",
    "$\\left|y\\right|\\le \\left|a\\right|$. Thus,\n",
    "\n",
    "$$\\  \\lim_{R\\to\\infty} \\left|\\int_{R-ia}^{R}e^{-R^2-2Ryi+y^2}\\, dy\\right| \\le \\lim_{R\\to\\infty} a^3 e^{a^2} e^{-R^2}=0.$$\n",
    "\n",
    "We may therefore conclude $\\left|I_2\\right|\\to0$ as $R\\to\\infty$ and\n",
    "furthermore, \n",
    "\n",
    "$$\\int_{c_2}e^{-z^2}\\, dz = \\int_{c_4}e^{-z^2}\\, dz = 0,$$\n",
    "\n",
    "as $R,L\\to\\infty$. Thus, we now have,\n",
    "\n",
    "$$\\ \\int_{c_1}e^{-z^2}\\, dz = \\int_{c_3}e^{-z^2}\\, dz = 0.$$ \n",
    "\n",
    "The integral over $c_3$ is, \n",
    "\n",
    "$$\\begin{aligned}\n",
    "    \\int_{c_3}e^{-z^2}\\, dz &= \\lim_{R,L\\to\\infty}\\int_{R}^{-L}e^{-z^2}\\, dz\\\\\n",
    "    &= \\lim_{R,L\\to\\infty}-\\int^{R}_{-L}e^{-z^2}\\, dz\\\\\n",
    "    &= -\\sqrt{\\pi},\n",
    "\\end{aligned}$$ \n",
    "\n",
    "Thus, we have finally proved,\n",
    "\n",
    "$$\\ \\int_{c_1}e^{-z^2}\\, dz = \\int_{-\\infty-\\frac{ix}{2\\sqrt{\\alpha t}}}^{\\infty-\\frac{ix}{2\\sqrt{\\alpha t}}}e^{-z^2}\\,dz = \\sqrt{\\pi}.$$"
   ]
  }
 ],
 "metadata": {
  "kernelspec": {
   "display_name": "Python 3 (ipykernel)",
   "language": "python",
   "name": "python3"
  },
  "language_info": {
   "codemirror_mode": {
    "name": "ipython",
    "version": 3
   },
   "file_extension": ".py",
   "mimetype": "text/x-python",
   "name": "python",
   "nbconvert_exporter": "python",
   "pygments_lexer": "ipython3",
   "version": "3.11.5"
  }
 },
 "nbformat": 4,
 "nbformat_minor": 5
}
